Clean-up and refactoring of the package imports

app/Main.hs
@@ -1,5 +1,10 @@
 module Main where
+import ENVCAP.Repl
+-- main :: IO ()
+-- main = do
+--   putStrLn "Starting App"
 
 main :: IO ()
 main = do
-  putStrLn "Starting App"
+  putStrLn "Welcome to the REPL! Type 'quit' or 'exit' to leave."
+  repl
